src/prop/PFStep.v
@@ -1,0 +1,95 @@
+Require Import Omega.
+Require Import RelationClasses.
+
+Require Import sflib.
+Require Import paco.
+
+Require Import Axioms.
+Require Import Basic.
+Require Import DataStructure.
+Require Import DenseOrder.
+Require Import Event.
+Require Import Time.
+Require Import Language.
+Require Import View.
+Require Import Cell.
+Require Import Memory.
+Require Import TView.
+Require Import Thread.
+
+
+Set Implicit Arguments.
+
+
+Inductive nonpf_step lang: forall (e:ThreadEvent.t) (e1 e2:Thread.t lang), Prop :=
+| nonpf_step_intro
+    st lc1 sc1 mem1
+    loc from to val released kind
+    lc2 mem2
+    (LOCAL: Local.promise_step lc1 mem1 loc from to val released lc2 mem2 kind)
+    (NONPF: Memory.op_kind_is_lower kind = false \/ released <> None):
+    nonpf_step (ThreadEvent.promise loc from to val released) (Thread.mk lang st lc1 sc1 mem1) (Thread.mk lang st lc2 sc1 mem2)
+.
+
+Inductive pf_step lang: forall (e:ThreadEvent.t) (e1 e2:Thread.t lang), Prop :=
+| step_pf_lower
+    st lc1 sc1 mem1
+    loc from to val kind
+    lc2 mem2
+    (LOCAL: Local.promise_step lc1 mem1 loc from to val None lc2 mem2 kind)
+    (KIND: Memory.op_kind_is_lower kind):
+    pf_step (ThreadEvent.promise loc from to val None) (Thread.mk lang st lc1 sc1 mem1) (Thread.mk lang st lc2 sc1 mem2)
+| step_pf_program
+    e e1 e2
+    (STEP: Thread.program_step e e1 e2):
+    pf_step e e1 e2
+.
+
+Lemma nonpf_step_future
+      lang e e1 e2
+      (STEP: @nonpf_step lang e e1 e2)
+      (WF1: Local.wf e1.(Thread.local) e1.(Thread.memory))
+      (SC1: Memory.closed_timemap e1.(Thread.sc) e1.(Thread.memory))
+      (CLOSED1: Memory.closed e1.(Thread.memory)):
+  <<WF2: Local.wf e2.(Thread.local) e2.(Thread.memory)>> /\
+  <<SC2: Memory.closed_timemap e2.(Thread.sc) e2.(Thread.memory)>> /\
+  <<CLOSED2: Memory.closed e2.(Thread.memory)>> /\
+  <<TVIEW_FUTURE: TView.le e1.(Thread.local).(Local.tview) e2.(Thread.local).(Local.tview)>> /\
+  <<SC_FUTURE: TimeMap.le e1.(Thread.sc) e2.(Thread.sc)>> /\
+  <<MEM_FUTURE: Memory.future e1.(Thread.memory) e2.(Thread.memory)>>.
+Proof.
+  inv STEP. ss. guardH NONPF.
+  exploit Local.promise_step_future; eauto. i. des.
+  splits; eauto. refl.
+Qed.
+
+Lemma pf_step_future
+      lang e e1 e2
+      (STEP: @pf_step lang e e1 e2)
+      (WF1: Local.wf e1.(Thread.local) e1.(Thread.memory))
+      (SC1: Memory.closed_timemap e1.(Thread.sc) e1.(Thread.memory))
+      (CLOSED1: Memory.closed e1.(Thread.memory)):
+  <<WF2: Local.wf e2.(Thread.local) e2.(Thread.memory)>> /\
+  <<SC2: Memory.closed_timemap e2.(Thread.sc) e2.(Thread.memory)>> /\
+  <<CLOSED2: Memory.closed e2.(Thread.memory)>> /\
+  <<TVIEW_FUTURE: TView.le e1.(Thread.local).(Local.tview) e2.(Thread.local).(Local.tview)>> /\
+  <<SC_FUTURE: TimeMap.le e1.(Thread.sc) e2.(Thread.sc)>> /\
+  <<MEM_FUTURE: Memory.future e1.(Thread.memory) e2.(Thread.memory)>>.
+Proof.
+  inv STEP; ss.
+  - exploit Local.promise_step_future; eauto. i. des.
+    splits; eauto. refl.
+  - eapply Thread.program_step_future; eauto.
+Qed.
+
+Lemma pf_step_dec
+      lang e e1 e2
+      (STEP: @Thread.step lang e e1 e2):
+  pf_step e e1 e2 \/ nonpf_step e e1 e2.
+Proof.
+  inv STEP.
+  - inv STEP0. destruct kind; try by right; econs; eauto.
+    destruct released; try by right; econs; eauto; right.
+    left. econs; eauto.
+  - left. econs 2. ss.
+Qed.
