src/prop/ReorderPromiseSame.v
@@ -23,6 +23,7 @@ Require Import SimLocal.
 Require Import FulfillStep.
 Require Import MemoryReorder.
 
+Require Import PFStep.
 Require Import PromiseConsistent.
 
 Set Implicit Arguments.
@@ -48,6 +49,67 @@ Proof.
   esplits; eauto.
   + econs; eauto.
   + econs; eauto.
+Qed.
+
+Lemma reorder_promise_promise_lower_None
+      lc0 mem0
+      lc1 mem1
+      lc2 mem2
+      loc1 from1 to1 val1 released1 kind1
+      loc2 from2 to2 val2 kind2
+      (STEP1: Local.promise_step lc0 mem0 loc1 from1 to1 val1 released1 lc1 mem1 kind1)
+      (STEP2: Local.promise_step lc1 mem1 loc2 from2 to2 val2 None lc2 mem2 kind2)
+      (LOCAL0: Local.wf lc0 mem0)
+      (MEM0: Memory.closed mem0)
+      (KIND2: Memory.op_kind_is_lower kind2 = true):
+  (loc1 = loc2 /\ from1 = from2 /\ to1 = to2 /\ val1 = val2 /\ kind2 = Memory.op_kind_lower released1 /\
+   exists kind1', <<STEP: Local.promise_step lc0 mem0 loc1 from1 to1 val1 None lc2 mem2 kind1'>>) \/
+  (exists lc1' mem1' from2' kind1',
+      <<STEP1: Local.promise_step lc0 mem0 loc2 from2' to2 val2 None lc1' mem1' kind2>> /\
+      <<STEP2: Local.promise_step lc1' mem1' loc1 from1 to1 val1 released1 lc2 mem2 kind1'>>).
+Proof.
+  inv STEP1. inv STEP2. ss. inv PROMISE0; inv KIND2. inv PROMISE.
+  - exploit MemoryReorder.add_lower; try exact PROMISES0; try exact PROMISES; eauto. i. des.
+    + subst.
+      exploit MemoryReorder.add_lower; try exact MEM1; try exact MEM; eauto. i. des; [|congr].
+      left. esplits; ss. econs; eauto. econs 1; eauto.
+    + exploit MemoryReorder.add_lower; try exact MEM1; try exact MEM; eauto. i. des; [congr|].
+      right. esplits.
+      * econs; [|by econs]. econs 3; eauto.
+      * refine (Local.step_promise _ _ _); eauto.
+        { econs 1; eauto. }
+        { eapply Memory.lower_closed_opt_view; eauto. }
+  - destruct (classic ((loc1, ts3) = (loc2, to2))).
+    { inv H.
+      exploit MemoryReorder.split_lower_same; try exact PROMISES0; try exact PROMISES; eauto. i. des.
+      exploit MemoryReorder.split_lower_same; try exact MEM1; try exact MEM; eauto. i. des.
+      subst. right. esplits.
+      - econs; [|by econs]. econs 3; eauto.
+      - refine (Local.step_promise _ _ _); eauto.
+        + econs 2; eauto.
+        + eapply Memory.lower_closed_opt_view; eauto.
+    }
+    { exploit MemoryReorder.split_lower_diff; try exact PROMISES0; try exact PROMISES; eauto. i. des.
+      - subst. exploit MemoryReorder.split_lower_diff; try exact MEM1; try exact MEM; eauto. i. des; [|congr].
+        left. esplits; eauto. econs; [|by econs]. econs 2; eauto.
+      - exploit MemoryReorder.split_lower_diff; try exact MEM1; try exact MEM; eauto. i. des; [congr|].
+        right. esplits; eauto.
+        + econs; [|by econs]. econs 3; eauto.
+        + refine (Local.step_promise _ _ _); eauto.
+          * econs 2; eauto.
+          * eapply Memory.lower_closed_opt_view; eauto.
+    }
+  - exploit MemoryReorder.lower_lower; try exact PROMISES0; try exact PROMISES; eauto. i. des.
+    + subst.
+      exploit MemoryReorder.lower_lower; try exact MEM1; try exact MEM; eauto. i. des; [|congr].
+      left. esplits; eauto.
+      econs; eauto. econs 3; eauto.
+    + exploit MemoryReorder.lower_lower; try exact MEM1; try exact MEM; eauto. i. des; [congr|].
+      right. esplits.
+      * econs; [|by econs]. econs 3; eauto.
+      * refine (Local.step_promise _ _ _); eauto.
+        { econs 3; eauto. }
+        { eapply Memory.lower_closed_opt_view; eauto. }
 Qed.
 
 Lemma reorder_promise_promise
@@ -200,10 +262,10 @@ Proof.
             - ii. inv H. eapply LOCTS; eauto.
           }
         * auto.
-    - exploit MemoryReorder.split_lower; try exact PROMISES; try exact PROMISES0; eauto.
+    - exploit MemoryReorder.split_lower_diff; try exact PROMISES; try exact PROMISES0; eauto.
       { ii. inv H. exploit LOCTS; eauto. i. des. congr. }
       i. des.
-      + subst. exploit MemoryReorder.split_lower; try exact MEM; try exact MEM0; eauto.
+      + subst. exploit MemoryReorder.split_lower_diff; try exact MEM; try exact MEM0; eauto.
         { ii. inv H. exploit LOCTS; eauto. i. des. congr. }
         i. des; [|congr].
         esplits.
@@ -212,7 +274,7 @@ Proof.
           { eapply REL_CLOSED. econs 2; eauto. }
         * left. auto.
         * congr.
-      + subst. exploit MemoryReorder.split_lower; try exact MEM; try exact MEM0; eauto.
+      + subst. exploit MemoryReorder.split_lower_diff; try exact MEM; try exact MEM0; eauto.
         { ii. inv H. exploit LOCTS; eauto. i. des. congr. }
         i. des; [congr|].
         esplits.
@@ -336,6 +398,29 @@ Proof.
     + econs; ss. econs; ss.
 Qed.
 
+      (* TODO *)
+      Lemma promise_step_nonsynch_loc_inv
+            lc1 mem1 loc from to val released lc2 mem2 kind l
+            (WF1: Local.wf lc1 mem1)
+            (STEP: Local.promise_step lc1 mem1 loc from to val released lc2 mem2 kind)
+            (NONPF: Memory.op_kind_is_lower kind = false \/ released <> None)
+            (NONSYNCH: Memory.nonsynch_loc l lc2.(Local.promises)):
+        Memory.nonsynch_loc l lc1.(Local.promises).
+      Proof.
+        guardH NONPF.
+        ii. destruct msg.
+        inv STEP. inv PROMISE; ss.
+        - exploit Memory.add_get1; try exact GET; eauto. i. des.
+          exploit NONSYNCH; eauto.
+        - exploit Memory.split_get1; try exact GET; eauto. i. des.
+          exploit NONSYNCH; eauto.
+        - exploit Memory.lower_o; try exact PROMISES; eauto.
+          instantiate (1 := t). instantiate (1 := l). condtac; ss.
+          + i. des. subst. exploit NONSYNCH; eauto. s. i. subst.
+            unguardH NONPF. des; congr.
+          + guardH o. rewrite GET. i. exploit NONSYNCH; eauto.
+      Qed.
+
 Lemma reorder_promise_write
       lc0 sc0 mem0
       lc1 mem1
@@ -344,6 +429,7 @@ Lemma reorder_promise_write
       loc2 from2 to2 val2 releasedm2 released2 ord2 kind2
       (STEP1: Local.promise_step lc0 mem0 loc1 from1 to1 val1 released1 lc1 mem1 kind1)
       (STEP2: Local.write_step lc1 sc0 mem1 loc2 from2 to2 val2 releasedm2 released2 ord2 lc2 sc2 mem2 kind2)
+      (NONPF: Memory.op_kind_is_lower kind1 = false \/ released1 <> None)
       (REL_WF: View.opt_wf releasedm2)
       (REL_CLOSED: Memory.closed_opt_view releasedm2 mem0)
       (LOCAL0: Local.wf lc0 mem0)
@@ -361,6 +447,7 @@ Lemma reorder_promise_write
                  exists from1' kind1', <<STEP2: Local.promise_step lc1' mem1' loc1 from1' to1 val1 released1 lc2 mem2 kind1'>>))>> /\
     <<KIND2: kind2 = Memory.op_kind_add -> kind2' = Memory.op_kind_add>>.
 Proof.
+  guardH NONPF.
   exploit Local.promise_step_future; eauto. i. des.
   exploit write_promise_fulfill; eauto; try by viewtac. i. des.
   exploit reorder_promise_promise; try exact STEP1; eauto.
@@ -386,22 +473,11 @@ Proof.
     exploit fulfill_step_future; try exact STEP7; try exact WF0; eauto; try by viewtac. i. des.
     exploit promise_fulfill_write_exact; try exact STEP4; eauto; try by viewtac.
     { i. exploit ORD; eauto. i. des. subst. splits; auto.
-      admit.
-
-  (* x : Memory.nonsynch_loc loc2 (Local.promises lc1) *)
-
-  (* STEP1 : Local.promise_step lc0 mem0 loc1 from1 to1 val1 released1 *)
-  (*           lc1 mem1 kind1 *)
-
-
-      (* apply Cell.ext. i. rewrite Cell.bot_get. *)
-      (* destruct (Cell.get ts (Local.promises lc0 loc2)) as [[? []]|] eqn:X; auto. *)
-      (* inv STEP1. exploit Memory.promise_promises_get1; eauto. i. des. *)
-      (* ss. unfold Memory.get in GET. rewrite x, Cell.bot_get in *. congr. *)
+      eapply promise_step_nonsynch_loc_inv; try exact STEP1; eauto.
     }
     { subst. inv STEP1. ss. }
     i. esplits; eauto. right. esplits; eauto.
-Admitted.
+Qed.
 
 Lemma reorder_promise_write'
       lc0 sc0 mem0
@@ -411,6 +487,7 @@ Lemma reorder_promise_write'
       loc2 from2 to2 val2 releasedm2 released2 ord2 kind2
       (STEP1: Local.promise_step lc0 mem0 loc1 from1 to1 val1 released1 lc1 mem1 kind1)
       (STEP2: Local.write_step lc1 sc0 mem1 loc2 from2 to2 val2 releasedm2 released2 ord2 lc2 sc2 mem2 kind2)
+      (NONPF: Memory.op_kind_is_lower kind1 = false \/ released1 <> None)
       (REL_WF: View.opt_wf releasedm2)
       (REL_CLOSED: Memory.closed_opt_view releasedm2 mem0)
       (LOCAL0: Local.wf lc0 mem0)
@@ -425,6 +502,7 @@ Lemma reorder_promise_write'
                   exists from1' kind1', <<STEP2: Local.promise_step lc1' mem1' loc1 from1' to1 val1 released1 lc2 mem2 kind1'>>))>> /\
      <<KIND2: kind2 = Memory.op_kind_add -> kind2' = Memory.op_kind_add>>).
 Proof.
+  guardH NONPF.
   destruct (classic (loc1 = loc2 /\ Time.lt to1 to2)); auto.
   right. eapply reorder_promise_write; eauto. i. subst. splits.
   - ii. subst. apply H. splits; auto.
@@ -438,24 +516,24 @@ Proof.
     + guardH o. des; congr.
 Qed.
 
-Lemma reorder_promise_program
+Lemma reorder_nonpf_program
       lang
       e1 e2 th0 th1 th2
-      (STEP1: @Thread.promise_step lang e1 th0 th1)
-      (STEP2: @Thread.program_step lang e2 th1 th2)
+      (STEP1: @nonpf_step lang e1 th0 th1)
+      (STEP2: Thread.program_step e2 th1 th2)
       (CONS2: promise_consistent th2.(Thread.local))
       (LOCAL: Local.wf th0.(Thread.local) th0.(Thread.memory))
       (SC: Memory.closed_timemap th0.(Thread.sc) th0.(Thread.memory))
       (MEMORY: Memory.closed th0.(Thread.memory)):
   exists th1',
-     <<STEP1: @Thread.program_step lang e2 th0 th1'>> /\
-     <<STEP2: __guard__ (th2 = th1' \/ exists e2', @Thread.promise_step lang e2' th1' th2)>>.
+     <<STEP1: Thread.program_step e2 th0 th1'>> /\
+     <<STEP2: __guard__ (th2 = th1' \/ exists e2', Thread.promise_step e2' th1' th2)>>.
 Proof.
-  exploit Thread.promise_step_future; eauto. i. des.
-  inv STEP1. inv STEP2; ss.
+  exploit nonpf_step_future; eauto. i. des.
+  inv STEP1. guardH NONPF. inv STEP2; ss.
   - (* silent *)
     esplits; eauto.
-    right. esplits. econs. eauto.
+    right. esplits. econs; eauto.
   - (* read *)
     exploit reorder_promise_read; try exact LOCAL0; eauto; try by viewtac.
     { ii. inv H.
@@ -492,19 +570,56 @@ Proof.
       exploit promise_consistent_promise_write; eauto. i.
       exfalso. eapply Time.lt_strorder. eapply TimeFacts.le_lt_lt; eauto.
     }
-    i. des. esplits.
+    esplits.
     + econs 4; eauto.
     + unguardH STEP3. des.
       * inv STEP3. left. auto.
       * right. esplits. econs; eauto.
   - inv LOCAL0. inv LOCAL1.
     esplits; eauto.
-    + econs 5; eauto. econs; eauto.
-      admit.
+    + econs 5; eauto. econs; eauto. ss.
+      intros ORDW l. eapply promise_step_nonsynch_loc_inv; eauto.
+      * econs; eauto.
+      * apply RELEASE. ss.
     + right. esplits. econs. econs; eauto.
   - inv LOCAL0. inv LOCAL1.
     esplits; eauto.
     + econs 6; eauto. econs; eauto.
-      admit.
+      intros ORDW l. eapply promise_step_nonsynch_loc_inv; eauto.
+      * econs; eauto.
+      * apply RELEASE. ss.
     + right. esplits. econs. econs; eauto.
-Admitted.
+Qed.
+
+Lemma reorder_nonpf_pf
+      lang
+      e1 e2 th0 th1 th2
+      (STEP1: @nonpf_step lang e1 th0 th1)
+      (STEP2: pf_step e2 th1 th2)
+      (CONS2: promise_consistent th2.(Thread.local))
+      (LOCAL: Local.wf th0.(Thread.local) th0.(Thread.memory))
+      (SC: Memory.closed_timemap th0.(Thread.sc) th0.(Thread.memory))
+      (MEMORY: Memory.closed th0.(Thread.memory)):
+  (exists e2',
+      <<STEP: Thread.step e2' th0 th2>> /\
+      <<EVENT: ThreadEvent.get_event e2' = ThreadEvent.get_event e2>>) \/
+  (exists e1' e2' th1',
+      <<STEP1: pf_step e1' th0 th1'>> /\
+      <<STEP2: Thread.promise_step e2' th1' th2>> /\
+      <<EVENT: ThreadEvent.get_event e1' = ThreadEvent.get_event e2>>).
+Proof.
+  inv STEP2; ss.
+  - inv STEP1. ss. guardH NONPF.
+    exploit reorder_promise_promise_lower_None; eauto. i. des.
+    + subst. left. esplits.
+      * econs 1. econs. eauto.
+      * ss.
+    + right. esplits.
+      * econs 1; eauto.
+      * econs. eauto.
+      * ss.
+  - exploit reorder_nonpf_program; eauto. i. des.
+    unguardH STEP2. des.
+    + subst. left. esplits; eauto.
+    + right. esplits; eauto. econs 2. ss.
+Qed.
